\subsection*{T3.55}
\subsubsection*{(a)}
\begin{align*}
f'(x) =e^{-h(x)}  \qquad \qquad f''(x) = -h'(x)e^{-h(x)}
\end{align*}
\paragraph{}
It is clear we have,
\begin{align*}
(f'(x))^2 \geq 0 \geq -h'(x) e^{-2h(x)}  =f''(x)f(x)
\end{align*}
\subsubsection*{(b)}
\paragraph{}
Take exponential and integrate both side of $e^{-h(t)} \leq e^{ -h(x) - h'(x) (t-x) }$
\begin{align*}
&\int_{-\infty}^{x}e^{-h(t)}dt \leq e^{xh'(x)-h(x)} \int_{-\infty}^{x}e^{-h'(x)t}dt \\
&\qquad \qquad \quad \ \ = e^{xh'(x)-h(x)}\frac{e^{-xh'(x)}}{-h'(x)} \\ 
&\qquad \qquad \quad \ \ = \frac{e^{-h(x)}}{-h'(x)}
\end{align*}
\paragraph{}
From here we have $-h'(x)e^{-h(x)}\int_{-\infty}^{x}e^{-h(t)}dt \leq e^{-2h(x)}$ which is just $f''(x)f(x) \leq (f'(x))^2$.