\subsection*{A4.26}
\subsubsection*{(a)}
\begin{align*}
&L(x,y,z) =\gamma||x||_1 +||y||_2 +z^T(Ax-b-y)\\
&\qquad \qquad =\gamma||x||_1 +z^TAx +(||y||_2-z^Ty) -b^Tz\\
&g(z)=\inf_{x,y}L(x,y,z) \\
&\qquad =\begin{cases}
&\inf_x(\gamma||x||_1+z^TAx-b^Tz), \qquad \text{if}\ ||z||_2 \leq 1\\
&-\infty \qquad \qquad \qquad \qquad \quad \ \ \text{otherwise}
\end{cases}\\
&\qquad =\begin{cases}
&-b^Tz, \qquad \text{if}\ ||A^Tz||_\infty \leq \gamma\\
&-\infty \qquad  \quad \text{otherwise}
\end{cases}
\end{align*}
\paragraph{}
Therefore the dual can be written as
\begin{align*}
&\text{maximize} \qquad -b^Tz\\
&\text{subject to} \qquad ||z||_2 \leq 1\\
&\qquad \qquad \qquad \ ||A^Tz||_\infty \leq \gamma
\end{align*}
\subsubsection*{(b)}
\paragraph{}
We examine the KKT conditions,
\begin{enumerate}
	\item $x,y \text{satisfy} Ax-b=y$
	\item $||A^Tz||_\infty \leq \gamma, ||z||_2 \leq 1$
	\item $x^\star, y^\star$ minimize $L(x,y,z^\star)$.
\end{enumerate}
\paragraph{}
Therefore for the last condition, we have
\begin{align*}
y^\star =\text{argmin}(||y||_2-y^Tz^\star) =0
\end{align*}
\paragraph{}
Therefore $z^\star = y^\star/||y^\star||_2 =(Ax^\star-b)/(||Ax^\star -b||_2)=r$, i.e., $r$ is dual optimal. and therefore we have
\begin{align*}
||A^Tr||_\infty \leq \gamma, \qquad r^TAx^\star +\gamma||x^\star||_1=0
\end{align*}
\paragraph{}
With the equation followed by strong duality.
\subsubsection*{(c)}
\paragraph{}
We write $A$ as followed,
\begin{align*}
A = \begin{bmatrix}
&a_1 &a_2 &\cdots &a_n
\end{bmatrix}
\end{align*}
\paragraph{}
Where $a_i \in R^m, i=1,...,n$.
\paragraph{}
From the strong duality
\begin{align*}
&(A^Tz)^Tx^\star+\gamma||x^\star||_1 = a_1^Tzx_1^\star + \cdots + a_n^Tzx_n^\star +\gamma(|x_1^\star|+\cdots+|x_n^\star|) \\
&\qquad \qquad \qquad \qquad \ = (a_1^Tzx_1^\star +\gamma|x_1^\star|)+...+(a_n^Tzx_n^\star +\gamma|x_n^\star|)\\
&\qquad \qquad \qquad \qquad \ \geq(-|a_1^Tz|x_1^\star +\gamma|x_1^\star|)+...+(-|a_n^Tz|x_n^\star +\gamma|x_n^\star|)\\
&\qquad \qquad \qquad \qquad \ \geq(-\gamma x_1^\star +\gamma|x_1^\star|)+...+(-\gamma x_n^\star +\gamma|x_n^\star|)\\
&\qquad \qquad \qquad \qquad \ =0
\end{align*}
\paragraph{}
Since $(A^Tz)^Tx^\star+\gamma||x^\star||_1 =0$. for the $i^{th}$ term we must either have $a_i^Tz = -|a_i^Tz| = -\gamma$ or $x_i=0$. Since $||a_i|| < \gamma$, we have $-|a_i^Tz| \leq -||a_i||||z|| < \gamma$ and therefore we must have $x_i=0$.
