\subsection*{T2.37}
\subsubsection*{(b)}
\paragraph{}
$\Rightarrow$
\paragraph{}
With $p(t) \geq 0$ we can rewrite it as:
\begin{align*}
&p(t) = r(t)^2 + s(t)^2 =
(r_1+r_2t+...+r_{k+1}t^k)^2 +(s_1+s_2t+...+s_{k+1}t^k)^2 \\
&\quad \ \ =(r_1^2 + s_1^2) +(r_1r_2+s_1s_2)t+...+(r_1r_{k+1}+s_1s_{k+1})t^k + \\
&\qquad \ \ \  (r_1r_2+s_1s_2)t+ (r_2^2 +s_2^2)t^2+...+(r_2r_{k+1}+s_2s_{k+1})t^{k+1} +\\
&\qquad \ \ \ ... \\
&\qquad \ \ + (r_1r_{k+1}+s_1s_{k+1})t^k + (r_2r_{k+1}+s_2s_{k+1})t^{k+1} +...+(r_{k+1}^2+s_{k+1}^2)t^{2k} \\
&\quad \ \ =\nu^tY\nu
\end{align*}
\paragraph{}
Where $\nu=[1, t, t^2 ... t^k] \in R^{k+1}$ and
\begin{align*}
Y=\begin{bmatrix*}[r]
r_1^2 + s_1^2        & r_1r_2+s_1s_2         & ... & r_1r_{k+1}+s_1s_{k+1} \\ 
r_1r_2+s_1s_2        & r_2^2 +s_2^2          & ... & r_2r_{k+1}+s_2s_{k+1} \\
...                  & ...                   & ... &...                    \\
r_1r_{k+1}+s_1s_{k+1}& r_2r_{k+1}+s_2s_{k+1} & ... & r_{k+1}^2+s_{k+1}^2   \\
\end{bmatrix*}
\end{align*}
\paragraph{}
Since $\nu^TY\nu \geq 0$, $Y\in S_+^{k+1}$. 
\paragraph{}
$\Leftarrow$
\paragraph{}
Conversely, with $x_i=\sum_{m+n=i+1}Y_{mn}$, we can rewrite $p(t)$ as
\begin{align*}
&p(t)= Y_{11} + (Y_{12}+Y_{21})t +(Y_{13}+Y_{22}+Y_{31})t^2 +...+Y_{k+1,k+1}t^{2k} \\
&\quad \ \  = \nu^tY\nu
\end{align*}
\paragraph{}
Where $\nu=[1, t, t^2 ... t^k] \in R^{k+1}$ and since $Y\in S_+^{k+1}$, we have $p(t) \geq 0$.
\subsubsection*{(c)}
\paragraph{}
From $K^{\ast}_{pol}=\{z \ | \ x^Tz \geq 0, \forall x\in K_{pol}\}$ we have
\begin{align*}
	\sum_{i=1}^{2k+1}z_i\sum_{m+n=i+1}Y_{mn}=\sum_{m,n=1}^{k+1}Y_{mn}z_{m+n-1}=\text{tr}(YH(z)) \geq 0	
\end{align*}
\paragraph{}
Therefore $H(z)\succeq 0$.
