\subsubsection*{A2.31}
\subsubsection*{(a)}
\paragraph{}
Using the composition rule, $f(x) =h(g(x))$ where $g(x)=||x||_2$, since $g(x)$ is convex on $R^n$ and $h(x)$ is nondecreasing and convex, $f(x)$ is convex.
\subsubsection*{(b)}
\paragraph{}
\begin{align*}
& f^{\ast}(y) = \sup_x(y^Tx -h(||x||_2))\\ 
&\qquad\ =\sup_{t\geq 0} \sup_{||x||_2 = t}(y^Tx - h(t)) \\ 
&\qquad\ \leq\sup_{t\geq 0} \sup_{||x||_2 = t}(||y||_2||x||_2 - h(t)) \\
&\qquad\ = \sup_{t\geq 0}(t||y||_2 - h(t)) \\
&\qquad\ = h^{\ast}(||y||_2)
\end{align*}
\subsubsection*{(c)}
\paragraph{}
Since$||y||_2 \geq 0$, we have
\begin{align*}
&h^{\ast}(||y||_2) =\sup_{t} (t||y||_2 - h(t)) \\
&\qquad \ \ \ \ \ \ = t||y||_2 - pt^p
\end{align*}
\paragraph{}
It reaches maximum at $||y||_2 = t^{p-1}$ and
\begin{align*}
f^{\ast}(y) = h^{\ast}(||y||_2) = \frac{p-1}{p}||y||_2^{\frac{p}{p-1}}, \qquad \forall y \in R^n
\end{align*}

