\subsection*{A2.5}
\paragraph{(a)}
from $g(x,t) =tf(x/t)$ we have
\begin{align*}
	&\frac{\partial g }{\partial t} =f(x/t) -\frac{x}{t}f(x/t) \\
	&\quad \ = f(x/t) +(0-\frac{x}{t})f(x/t) \leq f(0) \\
	&\quad \ \leq 0
\end{align*}
\paragraph{}
This is followed by first-order condition. Therefore $g(x,t)$ is nonincreasing as a function of $t$.
\paragraph{(b)}
\paragraph{}
We can write $h(x) = f(g(x,t))$, where $f(x,t) = tf(x/t)$ and $g(x,t) =g(x)$. From composition rule $g(x,t)$ is concave and $f(x,t)$ is nonincreasing and convex, hence $h(x)$ is convex.