\subsection*{A4.4}
\paragraph{}
We can rewrite the problem as
\begin{align*}
&minimize \qquad ||Az - b||_2^2\\
&subject\ to \qquad z^TCz + 2f^Tz = 0,
\end{align*}
\paragraph{}
where
\begin{align*}
A = \begin{bmatrix*}[r]
&-2y_1^T & 1 \\ &...&...\\&-2y_5^T&1\\
\end{bmatrix*} \qquad b = \begin{bmatrix*}[r]
&d_1^2 - ||y_1||^2_2 \\ &... \\&d_5^2 - ||y_5||^2_2 
\end{bmatrix*}\qquad C = \begin{bmatrix*}[r]
&1 &0 &0 \\&0 &1 &0\\ &0 &0 &0\\
\end{bmatrix*} \qquad f=\begin{bmatrix}
&0\\&0\\&-1/2
\end{bmatrix}
\end{align*}
\paragraph{}
The Lagrangian is
\begin{align*}
&L(z, \nu) = z^TA^TAz -2b^TAz+ b^Tb +\nu^T(z^TCz + 2f^Tz) \\
&\qquad \ \ \  =z^T(A^TA+\nu C)z - 2(A^Tb-\nu f)^Tz+b^Tb
\end{align*}
\paragraph{}
which is bounded below if
\begin{align*}
A^TA +\nu C \succeq 0 \qquad A^Tb -\nu f \in \text{Range}(A^TA +\nu C)
\end{align*}
\paragraph{}
and we have
\begin{align*}
&\triangledown L(z,v) = 2(A^TA + \nu C)z -2(A^Tb - \nu f) = 0 \Rightarrow  z = (A^TA+\nu C)^+(A^Tb-\nu f)
\end{align*}
\paragraph{}
Therefore $g(\nu)$ can be written as
\begin{align*}
g(\nu) = -(A^b-\nu f)^T(A^TA+\nu C)^+(A^Tb-\nu f) +b^Tb
\end{align*}{}
The dual can therefore be written as an SDP
\begin{align*}
&maximize \qquad -t +b^Tb\\
&subject\ to \qquad \begin{bmatrix*}[r]
&A^TA +\nu C &A^Tb- \nu f \\&(A^Tb-\nu f)^T &t 
\end{bmatrix*}\succeq 0
\end{align*}
\paragraph{}
This can be easily solved through CVX. This gives $\nu^{\star} =0.5896$, which gives $z^{\star} = [1.33, 0.64, 2.18]^T$. Therefore $x^{\star} = [1.33, 0.64]^T$.