\subsection*{T5.30}
\paragraph{}
With introduction of Lagrange multiplier $z \in R^n$, the KKT conditions are
\begin{enumerate}
	\item $X\succ 0$, 
	\item $Xs =y$,
	\item $X^{-1} = I +1/2(zs^T +sz^T)$,
\end{enumerate}
\paragraph{}
Combine 2 and 3 we have
\begin{align}
s = y +\frac{1}{2}(z+sz^Ty),
\end{align}
\paragraph{}
Multiplying $y^T$ on both side,
\begin{align*}
	1 -y^Ty =z^Ty
\end{align*}
\paragraph{}
Plugging it back to (1),
\begin{align*}
s = y +\frac{1}{2}(z+s-y^Tys) \Rightarrow z = (1+y^Ty)s -2y
\end{align*}
\paragraph{}
Plugging it back to 3 and we have
\begin{align*}
X^{-1} = I +(1+y^Ty)ss^T -ys^T-sy^T.
\end{align*}
\paragraph{}
To verify $X^\star = I +yy^T -ss^T/s^Ts$, 
\begin{align*}
&X^{-1}X^\star = (I +(1+y^Ty)ss^T -ys^T-sy^T)(I +yy^T -ss^T/s^Ts) \\
&\qquad \quad \ =I -yy^T -ss^T/s^Ts +(1+y^Ty)s^Ts +(1+y^Ty)sy^T \\
&\qquad \qquad -(1+y^Ty)s^Ts -ys^T-yy^T+ys^T-sy^T-y^Tysy^T+ss^T/s^Ts\\
&\qquad \quad \ = I
\end{align*}
\paragraph{}
Still we need to show $X^\star \succ 0$. This can be shown by
\begin{align*}
X^\star = I + yy^T - \frac{ss^T}{s^Ts} = (I+\frac{ys^T}{||s^Ts||_2}-\frac{ss^T}{s^Ts})(I+\frac{ys^T}{||s^Ts||_2}-\frac{ss^T}{s^Ts})^T \succ 0
\end{align*}
\paragraph{}
This is followed by the property of \textit{Cholesky Decomposition}.