\subsection*{Add.3}
\subsubsection*{(a)}
\paragraph{}
$\Rightarrow$
\paragraph{}
Provided that $X \in S^n$, We introduce $\nu = [\nu_1, \nu_k]^T$, where $\nu_1 \in R\ \text{and}\ \nu_k \in R^{n-1}$. Since $X \succeq 0$, we have
\begin{align*}
\nu X\nu =[\nu_1, \nu_k^T]\begin{bmatrix*}[r]
& 0 & B\\&B^T &C\\
\end{bmatrix*}\begin{bmatrix*}[r]
&\nu_1 \\&\nu_k\\ 
\end{bmatrix*}= \nu_k^TB^T\nu_1 + \nu_1B\nu_k +\nu_k^TC\nu_k \geq 0
\end{align*}
\paragraph{}
for any $\nu$. This is equivalent to $B =0$ and $C \succeq 0$.
\paragraph{}
$\Leftarrow$
\paragraph{}
Provided that $B =0$ and $C \succeq 0$, we can introduce $\nu = [\nu_1, \nu_k]^T$ and show $\nu X\nu \geq 0$.
\subsubsection*{(b)}
\begin{align*}
&AA^+ = [Q1 Q2]\begin{bmatrix*}[r]
&\Lambda_1 &0 \\&0 &0\\
\end{bmatrix*}\begin{bmatrix*}[r]
&Q^T_1 \\&Q^T_2 \\
\end{bmatrix*}Q_1\Lambda^{-1}_1Q_1^T = Q_1Q_1^T \\
&A^+A =Q_1\Lambda^{-1}_1Q_1^T[Q1 Q2]\begin{bmatrix*}[r]
&\Lambda_1 &0 \\&0 &0\\
\end{bmatrix*}\begin{bmatrix*}[r]
&Q^T_1 \\&Q^T_2 \\
\end{bmatrix*} =  Q_1Q_1^T
\end{align*}
\begin{align*}
I- AA^+ = I-A^+A = [Q_1\ Q_2]\begin{bmatrix*}[r]
&Q^T_1 \\&Q^T_2 \\
\end{bmatrix*} -  Q_1Q_1^T = Q_2Q_2^T
\end{align*}
\subsubsection*{(c)}
\paragraph{}
$\Rightarrow$
\paragraph{}
Assume $A \in S^n$ and $X \in S^{n+m}$. Introduce $\nu =  [\nu_1^T, \nu_2^T]$, where $\nu_1 \in R^n\ \text{and}\ \nu_2 \in R^m$. Since $X \succeq 0$, we have
\begin{align*}
\nu X\nu =[\nu_1^T, \nu_2^T]\begin{bmatrix*}[r]
& \Lambda & Q^TB\\&B^TQ &C\\
\end{bmatrix*}\begin{bmatrix*}[r]
&\nu_1 \\&\nu_2\\ 
\end{bmatrix*}= \nu_k^TB^T\nu_1 + \nu_1B\nu_1 +\nu_k^TC\nu_k \geq 0
\end{align*}