\subsection*{A3.21}
\subsubsection*{(a)}
\paragraph{}
Squaring both sides and use the observation in 4.26,
\begin{align*}
||\begin{bmatrix*}[r]
2y & z_1-z_2 \\
\end{bmatrix*}^T||_2 \leq z_1 +z_2
\end{align*}
\paragraph{}
Expand this and we have
\begin{align*}
4y^2 +z_1^2 +z^2_2 -2z_1z_2 \leq z_1^2 +z^2_2 +2z_1z_2
\end{align*}
\paragraph{}
This is just $y^2 \leq z_1z_2$. To extend this to the case where $n$ is a positive integer, first assume $n= 2^k$, and we have
\begin{align*}
&y^n \leq (y_{11}y_{12})^{2^k-1}\leq(y_{21}y_{22})^{2k-2}(y_{23}y_{24})^{2k-2} \\
&\quad \leq ...\leq (y_{k-1,1}y_{k-1, 2})^2(y_{k-1,3}y_{k-1, 4})^2...(y_{k-1,2^{k-1}-1}y_{k-1, 2^{k-1}})^2\\
&\quad \leq z_1z_2...z_{2^k},
\end{align*}
\paragraph{}
where we introduced variable $y_{ij},\ i=1,...,k-1, \ j=1,...,2^{k-1} $ and have the following inequalities:
\begin{align*}
&y_{k-1, j} \leq (z_{2j-1}z_{2j})^{1/2}, \qquad j = 1,...,2^{k-1} \\
&y_{i, j} \leq (y_{i+1,2j-1}y_{i+1,2j})^{1/2}, \qquad i= 1,...,k-2, j = 1,...,2^{i-1}
\end{align*}
\paragraph{}
With $ 2^k \leq n \leq 2^{k+1}$, we can write the original inequality as follow:
\begin{align*}
y^{2k+1} \leq y^{2k+1-n}z_1z_2...z_n
\end{align*}
\paragraph{}
and applied the same method above.
\subsubsection*{(b)}
We can express $\alpha$ as $p/q$, where $p,q>0$ since $\alpha$ is a rational number greater than 1, and the original inequality can be written as:
\begin{align*}
&x^{\alpha} = x^{p/q} \leq t \\
&x \leq t^{q/p} = (t^q)^{1/p}
\end{align*}
\paragraph{}
Now we can apply the same method in (a) by setting $z_1, z_2,...,z_{p-1} = 1\ \text{and}\ z_p =t^q$.
\paragraph{}
For the second function,