\subsection*{A3.11}
\subsubsection*{(a)}
\paragraph{}
The problem can be written as:
\begin{align*}
&\text{minimize} \qquad t \\
&\text{subject to} \qquad \begin{bmatrix*}[r]
&F(x) & c^T \\ & c & t\\
\end{bmatrix*} \succeq 0
\end{align*}
\paragraph{}
This is followed by \textit{Schur Component} with $t - c^TF^{-1}(x)c \geq 0$.
\subsubsection*{(b)}
\paragraph{}
The problem can be written as:
\begin{align*}
&\text{minimize} \qquad t \\
&\text{subject to} \qquad \begin{bmatrix*}[r]
&F(x) & c^T \\ & c & t\\
\end{bmatrix*} \succeq 0, \qquad i =1,...,K
\end{align*}
\subsubsection*{(c)}
\begin{align*}
f(x) =\lambda_{max}(F^{-1}(x)) \leq t \Leftrightarrow F^{-1}(x) \leq tI
\end{align*}
\paragraph{}
Therefore the problem is formed as followed
\begin{align*}
&\text{minimize} \qquad t \\
&\text{subject to} \qquad \begin{bmatrix*}[r]
&F(x) & I \\ & I & tI \\
\end{bmatrix*} \succeq 0
\end{align*}
\subsubsection*{(d)}
\begin{align*}
&E[c^TF^{-1}c] = E[\bar{c}^TF^{-1}\bar{c} + (c-\bar{c})^TF^{-1} (c-\bar{c})] \\
&\qquad \qquad \ \ =E[\bar{c}^TF^{-1}\bar{c}] + E[\sum_{i =1}^{m}\sum_{j =1}^{m}f_{ij}y_iy_j] \\
&\qquad \qquad \ \ =\bar{c}^TF^{-1}\bar{c} + \textbf{tr}(F^{-1}S)
\end{align*}
\paragraph{}
where $y_i = c_i -\bar{c_i}$. If we factor $S$ as $S = \sum_{k =1 }^{m} c_kc_k^T$ the problem is equivalent to 
\begin{align*}
minimize \qquad \bar{c}^TF^{-1}\bar{c} + \sum_{k =1 }^{m} c_k^TF(x)^{-1}c_k
\end{align*}
\paragraph{}
which is equivalent to 
\begin{align*}
&\text{minimize} \qquad t_0 +\sum_kt_k \\
&\text{subject to} \qquad \begin{bmatrix*}[r]
&F(x) & \bar{c}^T \\ & \bar{c}^T & t_0\\
\end{bmatrix*} \succeq 0 \\
&\qquad \qquad \qquad \ \begin{bmatrix*}[r]
&F(x) & c_k^T \\ & \ c_k^T & t_k\\
\end{bmatrix*} \succeq 0, \qquad k = 1,...,m
\end{align*}